---
tags:
  - math_172
  - integrals
  - trigonometry
---

> Three useful substitutions:
> $$ x = a \tan \theta, x = a \sin \theta, x = a \sec \theta $$
> These will be handy when integration something with the form $x^2 + a^2, a^2 - x^2, x^2 - a^2$.

Why use $x = a \tan \theta$ for $x^2 + a^2$?

![[8.4 Trigonometric Substitutions 2024-02-05 20.50.30.excalidraw]]

### Examples

> Find $\displaystyle \int \dfrac{x^2}{x^2 + 4} \, dx$.

Form: $x^2 + 2^2$

$x = 2 \tan \theta$
$dx = 2 \sec^2 \theta \, d \theta$

$= \displaystyle \int \dfrac{4 \tan^2 \theta}{4 \tan^2 \theta + 4} 2 \sec^2 \theta \, d \theta$
$= 2 \displaystyle \int \dfrac{\tan^2 \theta \sec^2 \theta}{\tan^2 \theta + 1} \, d \theta$
$= 2 \displaystyle \int \dfrac{\tan^2 \theta \sec^2 \theta}{\sec^2 \theta} \, d \theta$
$= 2 \int \tan^2 \theta \, d \theta$

- Note: $\tan^2 \theta = \sec^2 \theta - 1$

$= 2 \int (\sec^2 \theta - 1) \, d \theta$
$= 2(\tan \theta - \theta) + C$

$x = 2 \tan \theta$
$\frac{1}{2}x = \tan \theta$
$\tan^{-1}(\frac{1}{2}x) = \theta$

$= 2[\frac{1}{2}x - \tan^{-1}(\frac{1}{2}x)] + C$
$= x - 2 \tan^{-1}(\frac{1}{2}x) + C$

---

> Find $\displaystyle \int \dfrac{1}{x^2 \sqrt{9 - x^2}} \, dx$.

Form: $3^2 - x^2$

$x = 3 \sin \theta$
$dx = 3 \cos \theta \, d \theta$

$= \displaystyle \int \dfrac{3 \cos \theta}{9 \sin^2 \theta \sqrt{9 - 9 \sin^2 \theta}} \, d \theta$
$= \dfrac{1}{3} \displaystyle \int \dfrac{\cos \theta}{\sin^2 \theta \sqrt{9(1 - \sin^2 \theta)}} \, d \theta$
$= \dfrac{1}{9} \displaystyle \int \dfrac{\cos \theta}{\sin^2 \theta \sqrt{\cos^2 \theta}} \, d \theta$
$= \dfrac{1}{9} \displaystyle \int \dfrac{\cos \theta}{\sin^2 \theta \cos \theta} \, d \theta$
$= \dfrac{1}{9} \displaystyle \int \dfrac{1}{\sin^2 \theta} \, d \theta$
$= \frac{1}{9} \int \csc^2 \theta \, d \theta$
$= -\frac{1}{9} \cot \theta + C$

$\cot \theta = \dfrac{\text{adj}}{\text{opp}} = \dfrac{\sqrt{9 - x^2}}{x}$

$= -\dfrac{1}{9} \cdot \dfrac{\sqrt{9 - x^2}}{x} + C$
$= -\dfrac{\sqrt{9 - x^2}}{9x} + C$

---

> Find $\displaystyle \int_{5 \sqrt{2}}^{10} \dfrac{\sqrt{x^2 - 25}}{x} \, dx$.

$\dfrac{x}{5} = \sec \theta$ -> $\theta = \sec^{-1} \dfrac{x}{5}$
$\dfrac{5}{x} = \cos \theta$ -> $\theta = \sec^{-1} \dfrac{5}{x}$

$x = 5 \sec \theta$
$dx = 5 \sec \theta \tan \theta \, d \theta$
$x^2 = 25 \sec^2 \theta$

$x = 5 \sqrt{2}$ -> $\theta = \sec^{-1} \dfrac{5 \sqrt{2}}{5} = \cos^{-1} \dfrac{1}{\sqrt{2}} = \dfrac{1}{4} \pi$
$x = 10$ -> $\theta = \cos^{-1} \dfrac{5}{10} = \dfrac{1}{3} \pi$

$= \displaystyle \int_{\pi / 4}^{\pi / 3} \dfrac{\sqrt{25 \sec^2 \theta - 25}}{5 \sec \theta} 5 \sec \theta \tan \theta \, d \theta$
$= 5 \displaystyle \int_{\pi / 4}^{\pi / 3} \sqrt{\sec^2 \theta - 1} \tan \theta \, d \theta$
$= 5 \displaystyle \int_{\pi / 4}^{\pi / 3} \sqrt{\tan^2 \theta} \tan \theta \, d \theta$
$= 5 \displaystyle \int_{\pi / 4}^{\pi / 3} (\sec^2 \theta - 1) \, d \theta$
$= 5[\tan \theta - \theta]_{\pi / 4}^{\pi / 3}$
$= 5 [(\tan \frac{\pi}{3} - \frac{\pi}{3}) - (\tan \frac{\pi}{4} - \frac{\pi}{4})]$
$= 5 [\sqrt{3} - \frac{\pi}{3} - 1 + \frac{\pi}{4}]$
$= 5 [\sqrt{3} - 1 + \frac{\pi}{12}]$

---

> Find the area of the circle $x^2 + y^2 = a^2$.

$y = a^2 - x^2$ -> $y = \sqrt{a^2 - x^2}$

Find area of one quadrant, then multiply by 4:
$= 4 \displaystyle \int_0^a \sqrt{a^2 - x^2} \, dx$

$x = a \sin \theta$
$dx = a \cos \theta \, d \theta$
$x^2 = a^2 \sin^2 \theta$

$x = 0$ -> $\theta = \sin^{-1} 0 = 0$
$x = a$ -> $\theta = \sin^{-1} \dfrac{a}{a} = \dfrac{\pi}{2}$

$= 4 \displaystyle \int_0^{\pi / 2} \sqrt{a^2 - a^2 \sin^2 \theta} a \cos \theta \, d \theta$
$= 4a^2 \displaystyle \int_0^{\pi / 2} \sqrt{1 - \sin^2 \theta} \cos \theta \, d \theta$
$= 4a^2 \displaystyle \int_0^{\pi / 2} \sqrt{\cos^2 \theta} \cos \theta \, d \theta$
$= 4a^2 \displaystyle \int_0^{\pi / 2} \cos^2 \theta \, d \theta$

$\cos^2 \theta = \frac{1}{2}(1 + \cos(2 \theta))$

$= 4a^2 \displaystyle \int_0^{\pi / 2} \left[ \frac{1}{2}(1 + \cos(2 \theta)) \right] \, d \theta$
$= 2a^2 [\theta + \frac{1}{2} \sin(2 \theta)]_0^{\pi / 2}$
$= 2a^2 [(\frac{\pi}{2} + \frac{1}{2} \sin(2 \frac{\pi}{2})) - (0 + \frac{1}{2} \sin 0)]$
$= 2a^2 (\frac{\pi}{2})$
$= \pi a^2$