---
tags:
  - math_172
  - integrals
---

Recall: Common denominators

$$ \frac{1}{5} + \frac{2}{7} = \frac{7}{35} + \frac{10}{35} = \frac{17}{35} $$

In reverse: We can find $A$, $B$, such that

$$ \frac{17}{35} = \frac{A}{5} + \frac{B}{7} $$

$17 = 7A + 5B$

By inspection, one solution is $A = 1, B = 2$.

### Example

> Find $\displaystyle \int \dfrac{6}{x^2 - 1} \, dx$.

1. Factor the denominator into unique linear factors

$\dfrac{6}{x^2 - 1} = \dfrac{6}{(x + 1)(x - 1)}$

2. Assume there are constants $A$ and $B$ such that

$\dfrac{6}{x^2 - 1} = \dfrac{A}{x + 1} + \dfrac{B}{x - 1}$

3. Multiply by the largest denominator

$6 = (x - 1)A + (x + 1)B$

4. Find $A$ and $B$

- Note: pick easy values for $x$ (zeroing values)

Let $x = 1$
$6 = (1 - 1)A + (1 + 1)B$
$6 = 0A + 2B$
$B = 3$

Let $x = -1$
$6 = (-1 - 1)A + (-1 + 1)B$
$6 = -2A + 0B$
$A = -3$

5. Integrate

$\displaystyle \int \dfrac{6}{x^2 - 1} \, dx = \displaystyle \int \dfrac{-3}{x + 1} \, dx + \displaystyle \int \dfrac{3}{x - 1} \, dx$
$= -3 \ln |x + 1| + 3 \ln |x - 1| + C$

---

> The importance of *distinct* linear factors:

- Note: for $\frac{17}{35}$, there was only one way to factor 35.

But the denominator of $\frac{19}{40}$ has factors $2 \times 2 \times 2 \times 5$.

The decomposition of $\frac{19}{40}$ could have $\frac{1}{2}$, $\frac{1}{4}$, or $\frac{1}{8}$.

So try all of them!

### Examples

> Find $\displaystyle \int \dfrac{x^2 - x + 1}{(x + 1)^3} \, dx$.

Use all denominators:

$\dfrac{x^2 - x + 1}{(x + 1)^3} = \dfrac{A}{x + 1} + \dfrac{B}{(x + 1)^2} + \dfrac{C}{(x + 1)^3}$

$x^2 - x + 1 = (x + 1)^2 A + (x + 1)B + C$

Let $x = -1$
$(-1)^2 - (-1) + 1 = 0A + 0B + C$
$C = 3$

Let $x = 1$
$1^2 - 1 + 1 = (1 + 1)^2 A + (1 + 1)B + 3$
$1 = 4A + 2B + 3$
$-2 = 4A + 2B$

Let $x = 0$
$1 = A + B + 3$
$B = -2 - A$

Substitute and solve:

$-2 = 4A + 2(-2 - A)$
$A = 1$

$B = -2 - A$
$B = -3$

Alternatively: Find $A$, $B$, and $C$ by equating coefficients

$x^2 - x + 1 = (x^2 + 2x + 1)A + (x + 1)B + C$
$x^2 - x + 1 = Ax^2 + 2Ax + A + Bx + C + C$

Let's take a look at the $x^2$ terms:

$x^2 = Ax^2$
See that $A$ must be 1 here.

$-x = 2A + B$
$B = -3$

$1 - 1 + 3 = C$
$C = 3$

Plug in and solve:

$= \displaystyle \int \dfrac{1}{x + 1} \, dx - \displaystyle \int \dfrac{3}{(x + 1)^2} \, dx + \displaystyle \int \dfrac{3}{(x + 1)^3} \, dx$
$= \ln |x + 1| + \dfrac{3}{x + 1} - \dfrac{3}{2(x + 1)^2} + C$

---

## Improper rational functions

> A **proper rational function** has a denominator with a *greater* degree polynomial than its numerator.

This is an **improper rational function**:
$$ f(x) = \dfrac{x^2 + 2x - 5}{x^2 + x - 6} $$

Here, we will use polynomial long division to convert this to a sum of an integer and a proper rational function.

$\displaystyle \int \dfrac{x^2 + 2x - 5}{x^2 + x - 6}$
$= \displaystyle \int \left[ 1 + \dfrac{x + 1}{x^2 + x - 6} \right] \, dx$

### Example

> Find $\displaystyle \int \dfrac{6x^2 + 30}{x^3 + 6x} \, dx$.

- Note: $x^3 + 6x = x(x^2 + 6)$, which can't be reduced to (real) linear factors

Steps 1 and 2:

$\displaystyle \int \dfrac{6x^2 + 30}{x(x^2 + 6)} = \dfrac{A}{x} + \dfrac{Bx + C}{x^2 + 6}$

- Note: the $A$ term has an $x^0$, since it has to be 1 degree lower than $x^1$

Step 3:

$6x^2 + 30 = (x^2 + 6)A + x(Bx + C)$

Step 4:

$6x^2 + 30 = Ax^2 + 6A + Bx^2 + Cx$
Equate coefficients:
$x^2 \rightarrow 6 = A + B$
$x^1 \rightarrow 0 = C$
$x^0 \rightarrow 30 = 6A$

$A = 5, B = 1, C = 0$

$= \displaystyle \int \dfrac{5}{x} \, dx + \displaystyle \int \dfrac{x}{x^2 + 6} \, dx$

$= 5 \ln |x| + \frac{1}{2} \ln |x^2 + 6| + C$