---
tags:
  - math_172
  - series
---

For some values close to $x = 1$,
$$ \ln x = \sum_{k = 1}^\infty (-1)^{k + 1} \frac{(x - 1)^k}{k}. $$

This is a **power series**.
The form of a power series is:
$$ \sum_{k = 0}^\infty c_k (x - a)^k $$

---

It turns out that $\sum_{k = 1}^\infty (-1)^{k + 1} \dfrac{(x - 1)^k}{k}$ converges to $\ln x$ for $x \in (0, 2]$.
This interval is the **interval of convergence**.

Notice that the value $x = 1$ is the centre of the interval.
This is why $x = 1$ is the **centre** of this series.

The values $x = 0$ and $x = 2$ are the endpoints of the interval of convergence.
The distance from the centre to each endpoint is called the **radius of convergence (RoC)**.

## Finding the Interval of Convergence

We'll use the ratio test. For a power series $\sum_{k = 0}^\infty c_k (x - a)^k$,
compute the ratio
$$ \frac{c_{k + 1} (x - a)^{k + 1}}{c_k (x - a)^k} = \frac{c_{k + 1}}{c_k} (x - a) $$

Then find the limit of that:
$$ r = \lim_{k \to \infty} \Bigg| \frac{c_{k + 1}}{c_k} (x - a) \Bigg|. $$

According to the ratio test, the series converges when $0 \leq r < 1$. So solve the inequality $r < 1$.

Recall: Endpoints of the interval of convergence are $x = a \pm \text{RoC}$.

- If $\text{RoC} = \infty$, the series converges *everywhere*.
- If $\text{RoC} = 0$, the series converges only at $x = a$.
- We can't use this to determine convergence *at* the endpoints of the interval. We'll have to check those separately. (At the endpoints, $|r| = 1$, where the Ratio Test is inconclusive.)

> *Example*
> Find the radius of convergence and interval of convergence for
> $$ f(x) = \sum_{k = 1}^\infty \frac{(x + 3)^k}{k \cdot 2^k}. $$

Centre: $a = -3$
$c_k$ = $\dfrac{1}{k \cdot 2^k}$

$\lim_{k \to \infty} \left| \frac{c_{k + 1}}{c_k} (x - a) \right|$
$= \lim_{k \to \infty} \left| \frac{1}{(k + 1)2^k} \cdot \frac{k \cdot 2^k}{1} (x + 3) \right|$
$= |x + 3| \lim_{k \to \infty} \dfrac{1}{2k + 2}$
$= \dfrac{1}{2} |x + 3| = r$

Now, we need $|r| < 1$.

$\dfrac{1}{2} |x + 3| < 1$
$|x + 3| < 2$
$-2 < x + 3 < 2$
$-5 < x < -1$

RoC = 2
Endpoints: $x = -5$, $x = -1$

The interval of convergence is one of these choices:
- $(-5, -1)$
- $[-5, -1]$
- $(-5, -1]$
- $[-5, -1)$

We can test each of the endpoints:
$x = -5$:
$\displaystyle \sum_{k = 1}^\infty \dfrac{(-5 + 3)^k}{k \cdot 2^k}$
$= \sum_{k = 1}^\infty (-1)^k \frac{1}{k}$
This series converges (alternating harmonic series).

$x = -1$:
$\displaystyle \sum_{k = 1}^\infty \dfrac{(-1 + 3)^k}{k \cdot 2^k}$
$= \sum_{k = 1}^\infty \frac{1}{k}$
This series diverges (harmonic series).

Therefore, the interval of convergence is $[-5, -1)$.

---

Consider this power series:
$$ \sum_{k = 0}^\infty x^k = 1 + x + x^2 + x^3 + x^4 + \dots $$

How would we find
$$ \int \sum_{k = 0}^\infty x^k \, dx? $$

$\displaystyle \int \displaystyle \sum_{k = 0}^\infty \, dx = x + \dfrac{x^2}{2} + \dfrac{x^3}{3} + \dfrac{x^4}{4} + \dots + C$
$= \displaystyle \sum_{k = 0}^\infty \dfrac{x^{k + 1}}{k + 1} + C$

We can also think about the indefinite integral like this:
$= \displaystyle \sum_{k = 0}^\infty \displaystyle \int x^k \, dx$
$= \displaystyle \sum_{k = 0}^\infty \dfrac{x^{k + 1}}{k + 1} + C$

This power series is centred at $a = 0$.
This series is also a [[10.3 Infinite Series|geometric series]] and thus converges when $|x| < 1$.

The interval of convergence is $I = (-1, 1)$. Since the Geometric Series Test isn't inconclusive at $|r| = 1$, we don't need to check the endpoints.
The radius of convergence is $\text{RoC} = 1$.
When $x \in I$, the series converges to $\dfrac{a}{1 - r} = \dfrac{1}{1 - x}$. ($a$ is the first term, not the centre.)

> *Example*
> Find the radius of convergence and interval of convergence for the power series for $f(x) = \dfrac{1}{5 - x}$.

- Note: This is similar to the original geometric series result $\dfrac{1}{1 - x}$

$\dfrac{1}{5 - x} = \dfrac{\frac{1}{5}}{1 - \frac{x}{5}}$
This is still a geometric series, with $a = \frac{1}{5}$ and $r = \frac{x}{5}$.

$\dfrac{1}{5 - x} = \displaystyle \sum_{k = 0}^\infty \dfrac{1}{5} \left( \dfrac{x}{5} \right)^k$
$=\dfrac{1}{5} \displaystyle \sum_{k = 0}^\infty \left( \dfrac{x}{5} \right)^k$

Centre: $x = 0$
Interval of convergence:
$\left| \dfrac{x}{5} \right| < 1$
$|x| < 5$
$-5 < x < 5$
$I = (-5, 5)$
Radius of convergence: 5

> *Example*
> Find a power series representation for $f(x) = \ln|5 - x|$.

- Note: $\dfrac{d}{dx} \ln|5 - x| = -\dfrac{1}{5 - x}$

$-\displaystyle \int \dfrac{1}{5 - x} \, dx = \ln|5 - x| + C$
$= -\displaystyle \int \displaystyle \sum_{k = 0}^\infty \dfrac{x^k}{5^{k + 1}} \, dx$
$= -\displaystyle \sum_{k = 0}^\infty \dfrac{x^k}{5^{k + 1}} \displaystyle \int x^k \, dx$
$= -\displaystyle \sum_{k = 0}^\infty \dfrac{1}{5^{k + 1}} \cdot \dfrac{x^{k + 1}}{k + 1} + C$
$= -\displaystyle \sum_{k = 0}^\infty \dfrac{x^{k + 1}}{5^{k + 1} (k + 1)} + C$

Now, we just need to find $C$.

We will evaluate at $x = 0$ (the centre of the series):
$\ln|5 - 0| = -\displaystyle \sum_{k = 0}^\infty \dfrac{0^{k + 1}}{5^{k + 1} (k + 1)} + C$
$\ln 5 = -0 + C$
$C = \ln 5$

Therefore,
$$ \ln|5 - x| = -\sum_{k = 0}^\infty \dfrac{x^{k + 1}}{5^{k + 1} (k + 1)} + \ln 5 $$

- Note: The interval of convergence is the same as the original series: $I = (-5, 5)$

Applying integrals and derivatives do not change the interval of convergence and radius of convergence.