---
tags:
  - math_172
  - series
---

> A **Taylor Series** is an infinite-degree Taylor polynomial - a special case of a power series. A Taylor Series centred at 0 is a **Maclaurin Series**.

> *Example*
> Find the Maclaurin Series for $f(x) = e^x$.

| k   | $f^{(k)}(x) | f^{(k)}(a) | $\times$ | $1 / k!$ | $=$ | $c_k$    |
| --- | ----------- | ---------- | -------- | -------- | --- | -------- |
| 0   | $e^x$       | 1          | $\times$ | $1 / 0!$ | $=$ | $1 / 0!$ |
| 1   | $e^x$       | 1          | $\times$ | $1 / 1!$ | $=$ | $1 / 1!$ |
| 2   | $e^x$       | 1          | $\times$ | $1 / 2!$ | $=$ | $1 / 2!$ |
| 3   | $e^x$       | 1          | $\times$ | $1 / 3!$ | $=$ | $1 / 3!$ |

$$ f(x) = e^x = \frac{1}{0!}(x - 0)^0 + \frac{1}{1!}(x - 0)^1 + \frac{1}{2!}(x - 0)^2 + \frac{1}{3!}(x - 0)^3 + \dots $$
$$ e^x = \sum_{k = 0}^\infty \frac{x^k}{k!} $$

Find the interval of convergence:

Use the Ratio Test:
$r = \displaystyle \lim_{k \to \infty} \left| \dfrac{\dfrac{x^{k + 1}}{(k + 1)!}}{\dfrac{x^k}{k!}} \right|$
$= \displaystyle \lim_{k \to \infty} \left| \dfrac{x^{k + 1}}{(k + 1)!} \cdot \dfrac{k!}{x^k} \right|$
$= \displaystyle \lim_{k \to \infty} \left| \dfrac{x}{k + 1} \right|$
$= |x| \displaystyle \lim_{k \to \infty} \dfrac{1}{k + 1}$
$= 0$

Solving $0 < 1$, all values of $x$ make this inequality true.

RoC: $\infty$
IoC: $x \in (-\infty, \infty)$

> *Example*
> Find the $n$th-degree Taylor polynomial for $f(x) = x^4$ (With $n \geq 4$).

| k   | $f^{(k)}(x) | f^{(k)}(a) | $\times$ | $1 / k!$ | $=$ | $c_k$           |
| --- | ----------- | ---------- | -------- | -------- | --- | --------------- |
| 0   | $x^4$       | 0          | $\times$ | $1 / 0!$ | $=$ | $0!$            |
| 1   | $4x^3$      | 0          | $\times$ | $1 / 1!$ | $=$ | $0$             |
| 2   | $12x^2$     | 0          | $\times$ | $1 / 2!$ | $=$ | $0$             |
| 3   | $24x$       | 0          | $\times$ | $1 / 3!$ | $=$ | $0$             |
| 4   | $24$        | 24         | $\times$ | $1 / 4!$ | $=$ | $24 / (4!) = 1$ |
| 5   | $0$         | 0          | $\times$ | $1 / 5!$ | $=$ | $0!$            |

Therefore, $x^4 = 1(x - 0)^4 = x^4$.

> *Example*
> Find the Maclaurin Series for $f(x) = x^4 e^{-3x^2}$.

Note that the Maclaurin Series for $f(x) = e^x$ is $\displaystyle \sum_{k = 0}^\infty \dfrac{x^k}{k!}$.
So, $e^{-3x^2} = \displaystyle \sum_{k = 0}^\infty \dfrac{(-3x^2)^k}{k!}$
$= \displaystyle \sum_{k = 0}^\infty \dfrac{(-1)^k 3^k x^{2k}}{k!}$

$x^4 e^{-3x^2} = x^4 \displaystyle \sum_{k = 0}^\infty \dfrac{(-1)^k 3^k x^{2k}}{k!}$
$= \displaystyle \sum_{k = 0}^\infty \dfrac{(-1)^k 3^k x^{2k + 4}}{k!}$