---
tags:
  - math_172
  - series
---

We know that the Harmonic Series $\displaystyle \sum_{k = 1}^\infty \dfrac{1}{k}$ diverges.

What about $\displaystyle \sum_{k = 1}^\infty \dfrac{(-1)^{k + 1}}{k}$?

The first few terms: $1 - \frac{1}{2} + \frac{1}{3} - \frac{1}{4}$

In general, any series with alternating signs (a factor in the form $(-1)^k$ or $(-1)^{k + 1}$) is called an **alternating series**.

> *Theorem 10.16: The Alternating Series Test*
> The alternating series $\sum (-1)^{k + 1} a_k$ converges provided
> 1. the terms of the series are non-increasing in magnitude ($0 < a_{k + 1} \leq a_k$ for $k$ greater than some index $N$) and
> 2. $\lim_{k \to \infty} a_k = 0$

- Note: the Alternating Series Test is the only one that can be used to show **convergence** of an alternating series

### Examples

> Is the following series convergent or divergent?
> $$ \sum_{k = 1}^\infty \frac{(-1)^{k + 1}}{k} $$

$a_k = \dfrac{1}{k}$

1. Are the terms of $a_k$ eventually non-increasing?

$\dfrac{1}{k} > \dfrac{1}{k + 1}$, so $a_k$ is decreasing.

3. Is $\lim_{k \to \infty} a_k = 0$?

$\lim_{k \to \infty} \dfrac{1}{k} = 0$

By the Alternating Series Test, the given series converges.

---

> Is the following series convergent or divergent?
> $$ \sum_{k = 1}^\infty (-1)^{k + 1} \frac{1}{k^4} $$

$a_k = \dfrac{1}{k^4}$

Since the terms of $a_k$ are decreasing, and $\lim_{k \to \infty} a_k = 0$, by the Alternating Series Test, the given series converges.