---
tags:
  - math_172
  - polar
---

If $r = f(\theta)$, then

$x = r \cos \theta$ -> $\dfrac{dx}{d \theta} = \dfrac{dr}{d \theta} \cos \theta + r(-\sin \theta)$
$y = r \sin \theta$ -> $\dfrac{dy}{d \theta} = \dfrac{dr}{d \theta} \sin \theta + r(\cos \theta)$

So,
$$ \frac{dy}{dx} = \frac{\frac{dr}{d \theta} \sin \theta + r \cos \theta}{\frac{dr}{d \theta} \cos \theta - r \sin \theta} $$

$\dfrac{dy}{dx} = \dfrac{\cos \theta \sin \theta + (1 + \sin \theta) \cos \theta}{\cos \theta \cos \theta - (1 + \sin \theta) \sin \theta}$
$\dfrac{dy}{dx} = \dfrac{\cos \theta (1 + 2 \sin \theta)}{\cos^2 \theta - \sin \theta - \sin^2 \theta}$

Solve:
$\cos \theta (1 + 2 \sin \theta) = 0$
1. $\cos \theta = 0$
$\theta = \dfrac{\pi}{2}, \dfrac{3 \pi}{2}$

2. $1 + 2 \sin \theta = 0$
$2 \sin \theta = -1$
$\sin \theta = -\dfrac{1}{2}$
$\theta = \dfrac{7 \pi}{6}, \dfrac{11 \pi}{6}$

These are candidates for a horizontal tangent, but we need to verify that the denominator is not 0 for these candidates.

$\cos^2 \theta - \sin \theta - \sin^2 \theta = (1 - 2 \sin \theta)(1 + \sin \theta)$

We need to avoid $(1 - 2 \sin \theta)(1 + \sin \theta) = 0$.