---
tags:
  - math_172
---

> Finding the length of a curve using integrals.

Since $f'(x) = \dfrac{\Delta y}{\Delta x}$, $\Delta y = f'(x) \Delta x$.

![[6.5 Arc Length 2024-01-22 09.44.47.excalidraw]]

The length of the hypotenuse of $\Delta x$ and $\Delta y$ is
$L = \sqrt{(\Delta x)^2 + (\Delta y)^2}$
$= \sqrt{(\Delta x)^2 + [f'(x) \Delta x]^2}$
$= \sqrt{(\Delta x)^2 (1 + [f'(x)^2])}$
$= \sqrt{1 + [f'(x)]^2} \Delta x$

The sum of these lengths will give us the total arc length:

> $$ L = \int_a^b \sqrt{1 + [f'(x)]^2} \, dx $$

### Examples

> Find the length of the curve $y = x$ from $x = 0$ to $x = 1$.

$f'(x) = 1$
$L = \displaystyle \int_0^1 \sqrt{1 + 1^2} \, dx$
$= \displaystyle \int_0^1 \sqrt{2} \, dx$
$= \sqrt{2}$

---

> Find the length of the curve $f(x) = \dfrac{x^3}{6} + \dfrac{1}{2x}$ from $x = 1$ to $x = 3$.

$f'(x) = \dfrac{x^2}{2} - \dfrac{1}{2x^2}$
$[f'(x)]^2 = \dfrac{x^4}{4} - \dfrac{1}{2} + \dfrac{1}{4x^4}$
$L = \displaystyle \int_1^3 \displaystyle \sqrt{1 + \left[ \dfrac{x^4}{4} - \dfrac{1}{2} + \dfrac{1}{4x^4} \right]} \, dx$
$= \displaystyle \int_1^3 \displaystyle \sqrt{\dfrac{x^4}{4} + \dfrac{1}{2} + \dfrac{1}{4x^4}} \, dx$
$= \displaystyle \int_1^3 \displaystyle \sqrt{\left( \dfrac{x^2}{2} + \dfrac{1}{2x^2} \right)^2} \, dx$
$= \displaystyle \int_1^3 \left( \dfrac{x^2}{2} + \dfrac{1}{2x^2} \right) \, dx$
$= \dfrac{14}{3}$

---

> Find the length of the curve $y^3 = x^2$ from $(0, 0)$ to $(1, 1)$.

```desmos-graph
left = -1.5; right = 1.5;
top = 1.5; bottom = -1.5;
---
y^3 = x^2
y^3 = x^2 | 0 <= x <= 1 | red
```

- Note: we can solve this in terms of $x$ instead of $y$

$g(y) = x = y^\frac{3}{2}$
$g'(y) = \dfrac{3}{2}y^\frac{1}{2}$
$[g'(y)]^2 = \dfrac{9}{4}y$

$L = \displaystyle \int_0^1 \sqrt{1 + \dfrac{9}{4}y}
 \, dy$

Let $u = 1 + \dfrac{9}{4}y$
$\dfrac{du}{dy} = \dfrac{9}{4}$ -> $dy = \dfrac{4}{9}du$
$u(0) = 1, u(1) = \dfrac{13}{4}$

$= \dfrac{4}{9} \displaystyle \int_1^\frac{13}{4} u^{\frac{1}{2}} \, du$
$= \dfrac{4}{9} \left[ \dfrac{2}{3}u^\frac{3}{2} \right]_1^\frac{13}{4}$
$\dfrac{1}{27} (13^\frac{3}{2} - 8)$