#math_171 #derivatives 

Consider:

| $f(x)$ | $f'(x)$ |
| ------ | ------- |
| $x^0$  | $0x^-1$ |
| $x^1$  | $1x^0$  |
| $x^2$  | $2x^1$  |
| $x^3$  | $3x^2$  |
| $x^4$  | $4x^3$  |

> *Theorem 3.3: Power Rule*
> If $n$ is a non-negative integer, then $\frac{d}{dx} (x^n) = nx^{n - 1}$.

(Actually, $n$ can be any real number)

> *Theorem 3.2: Constant Rule*
> If $c$ is a real number, then $\frac{d}{dx} (c) = 0$.

> *Theorem 3.4: Constant Multiple Rule*
> If $f$ is differentiable at $x$ and $c$ is a constant, then
> $$ \frac{d}{dx} (cf(x)) = cf'(x). $$

> *Theorem 3.5: Sum Rule*
> If $f$ and $g$ are differentiable at $x$, then
> $$ \frac{d}{dx} (f(x) + g(x)) = f'(x) + g'(x). $$

## Derivative of $e^x$

For $f(x) = e^x$, $f'(x) = e^x$.

This means that the slope at any point of $f(x)$ is the value of $f(x)$.

### Example

> Find the equation of the line that is tangent to the graph of $y = x^3 + \frac{e^x}{2}$ at the point where $x = 1$.

At $x = 1$, $y = (1)^3 + \frac{e^{(1)}}{2}$ = $1 + \frac{e}{2}$.

Derivative:
$y' = \frac{dy}{dx} = \frac{d}{dx} (x^3 + \frac{1}{2} e^x)$
$y' = 3x^2 + \frac{1}{2}e^x$

Slope at $x = 1$:
$y' = 3(1)^2 + \frac{e^{(1)}}{2} = 3 + \frac{e}{2}$

Equation of line:
$y - (1 + \frac{e}{2}) = (3 + \frac{e}{2})(x - 1)$

## Higher order derivatives

$$ f(x) \rightarrow f'(x) \rightarrow f''(x) \rightarrow f'''(x) \rightarrow \dots \rightarrow f^{(10)}(x) $$

$$ y'' = \frac{d^2y}{dx^2} = \frac{d^2}{dx^2} (y) $$

### Example

> Find $f'(x)$, $f''(x)$, and $f'''(x)$ for $f(x) = 3x^3 + 5x^2 + 6x$.

$f'(x) = \frac{d}{dx} (f(x)) = 9x^2 + 10x + 6$
$f''(x) = \frac{d}{dx} (f'(x)) = 18x + 10$
$f'''(x) = \frac{d}{dx} (f''(x)) = 18$