#math_171 

> *Theorem 3.13: The Chain Rule*
> Suppose $y = f(u)$ is differentiable at $u = g(x)$ and $u = g(x)$ is differentiable at $x$. The composite function $y = f(g(x))$ is differentiable at $x$, and its derivative can be expressed in two equivalent ways.
> 1. $$ \frac{dy}{dx} = \frac{dy}{du} \cdot \frac{du}{dx} $$
> 2. $$ \frac{dy}{dx} = f'(g(x)) \cdot g'(x) $$

## Function decomposition

Think of $y = f(g(x))$ as:
- $y = f(u)$
- $u = g(x)$

So, $\frac{\Delta y}{\Delta x} = \frac{\Delta y}{\Delta u} \cdot \frac{\Delta u}{\Delta x}$
As $\Delta x \to 0$, $\frac{dy}{dx} = \frac{dy}{du} \cdot \frac{du}{dx}$

$\frac{dy}{du}$ is evaluated at the $u$ value $u = g(x)$.

This is one version of the Chain Rule.

#### Intuitive explanation

- $y$ is dollars
- $u$ is number of units
- $x$ is hours
-> $\frac{\$}{hr} = \frac{\$}{unit} \cdot \frac{units}{hr}$

### Alternative version

Given $y = f(u)$ and $u = g(x)$,
$$ \frac{dy}{dx} = f'(g(x)) \cdot g'(x) $$

Or:
$$ \frac{d}{dx} (f(\fbox{})) = f'(\fbox{}) \cdot \fbox{}' $$

## Examples

> Find $\frac{dy}{dx}$ if $y = (4x^2 + 8x)^{12}$.

$\frac{dy}{dx} = \frac{d}{dx} ((4x^2 + 8x)^{12})$
$= 12(4x^2 + 8x)^{11} \cdot (8x + 8)$

> Find $\frac{dy}{dx}$ if $y = \sin(\sin(e^x))$.

$y' = \frac{d}{dx} (\sin(\sin(e^x)))$
$= \cos(\sin(e^x)) \cdot \frac{d}{dx} (\sin(e^x))$
$= \cos(\sin(e^x)) \cdot \cos(e^x) \cdot e^x$