---
tags:
  - math_171
  - integrals
---

The substitution rule is the "reversal" of the [[3.7 The Chain Rule|chain rule]].

Idea:
$\frac{d}{dx} (\sin(x^3)) = \cos(x^3) \cdot 3x^2$,
so it follows that
$\int 3x^2 \cos(x^3) \, dx = \sin(x^3) + C$.

### Example

> $\int x^2 \cos(x^3) \, dx$

$= \int \frac{1}{3} \cdot 3x^2 \cos(x^3) \, dx$
$= \frac{1}{3} \int 3x^2 \cos(x^3) \, dx$
$= \frac{1}{3} \sin(x^3)$

---

> *Theorem 5.7: Substitution Rule for Definite Integrals*
> Let $u = g(x)$, where $g'$ is continuous on $[a, b]$, and let $f$ be continuous on the range of $g$. Then
> $$ \int_a^b f(g(x)) g'(x) \, dx = \int_{g(a)}^{g(b)} f(u) du. $$