#math_171 

> *Theorem 2.2: Limits of Linear Functions*
> Let $a$, $b$, and $m$ be real numbers. For linear functions $f(x) = mx + b$,
> $$ \lim_{x \to a} f(x) = f(a) = ma + b $$
> In other words, $\lim_{x \to a} (mx + b) = ma + b$
> This is known as *direct substitution*.
> - Note: a linear function has a line as its graph; there are no holes, so direct substitution always works


> *Theorem 2.3: Limit Laws*
> Assume $\lim_{x \to a} f(x)$ and $\lim_{x \to a} g(x)$ exist. The following properties hold, where $c$ is a real number, and $n > 0$ is an integer:
> 1. **Sum**: $\lim_{x \to a} (f(x) + g(x)) = \lim_{x \to a} f(x) + \lim_{x \to a}$
> 2. **Difference**: $\lim_{x \to a} (f(x) - g(x)) = \lim_{x \to a} f(x) - \lim_{x \to a}$
> 3. **Constant multiple**: $\lim_{x \to a} (cf(x)) = c \lim_{x \to a} f(x)$
> 4. **Product**: $\lim_{x \to a} (f(x)g(x)) = (\lim_{x \to a} f(x))(\lim_{x \to a} g(x))$
> 5. **Quotient**: $\lim_{x \to a} \frac{f(x)}{g(x)} = \frac{\lim_{x \to a} f(x)}{\lim_{x \to a} g(x)}$, provided $\lim_{x \to a} g(x) \neq 0$
> 6. **Power**: $\lim_{x \to a} (f(x))^n = (\lim_{x \to a} f(x))^n$
> 7. **Root**: $\lim_{x \to a} (f(x))^\frac{1}{n} = (\lim_{x \to a} f(x))^\frac{1}{n}$, provided $f(x) \geq 0$, for $x$ near $a$, if $n$ is even (from *BOTH* sides)
> - Note: some cases for quotients and roots will be undefined, so make sure the function is defined for values of $x$ near $a$
> - Note: the root rule always works when $n$ is odd

> *Theorem 2.4: Limits of Polynomial and Rational Functions*
> 1. **Polynomial functions**: $\lim_{x \to a} p(x) = p(a)$
> 2. **Rational functions**: $\lim_{x \to a} \frac{p(x)}{q(x)} = \frac{p(a)}{q(a)}$
> 
> In other words, direct substitution works for polynomial functions and for rational functions (provided the denominator does not approach 0)

> If $f(x) = g(x)$ for all $x$ near $a$ (not necessarily at $x = a$), then $\lim_{x \to a} f(x) = \lim_{x \to a} g(x)$

### Example

> Find $\lim_{x \to -2} (4x + 11)$

We can just plug in -2 for $x$:
$$ \lim_{x \to -2} (4x + 11) = 4(-2) + 11 = 3 $$

- Note: direct substitution does not always work for finding a limit

For example, $\lim_{x \to 0} \frac{x}{x^2 - 2x}$ is undefined for $x = 0$

## Special cases

Two special cases of $\lim_{x \to a} (mx + b) = ma + b$:

1. $\lim_{x \to a} (b) = b$
	- The outputs stay at $b$ the whole time
2. $\lim_{x \to a} (mx) = ma$

### Example

> Find $\lim_{x \to 4} (8x)$

Special case #2: $\lim_{x \to 4} (8x) = 8(4) = 32$

## Laws

If $\lim_{x \to a} f(x) = L$ and $\lim_{x \to a} g(x) = M$, then
$$ \lim_{x \to a} \frac{f(x)}{g(x)} = \frac{L}{M} $$

### Examples

> Find $\lim_{x \to 3} \frac{x}{2x + 1}$

Using the above law: $\lim_{x \to 3} \frac{x}{2x + 1} = \frac{3}{2(3) + 1} = \frac{3}{7}$

> Find $\lim_{t \to -2} (t^2 + 5t + 7)$

$(-2)^2 + 5(-2) + 7 = 1$

> Find $\lim_{x \to 2} \sqrt{4x - 8}$

When $x$ approaches 2 from the right, $4x - 8 > 0$, but when $x$ approaches 2 from the left, $4x - 8 < 0$. Therefore, $\lim_{x \to 2} \sqrt{4x - 8}$ DNE, but $\lim_{x \to 2^+} \sqrt{4x - 8} = 0$