---
tags:
  - math_172
  - trigonometry
---

Given $x^2 + y^2 = 1$,
We can relate $\cos t$ and $\sin t$ with a *Pythagorean identity*:

$$ \sin^2 t + \cos^2 t = 1 $$

## Hyperbolic functions

Similarly, we can relate hyperbolic functions to hyperbolas, i.e. $x^2 - y^2 = 1$

- $\cosh t = \dfrac{e^t + e^{-t}}{2}$
- $\sinh t = \dfrac{e^t - e^{-t}}{2}$
- $\tanh x = \dfrac{\sinh x}{\cosh x} = \dfrac{e^x - e^{-x}}{e^x + e^{-x}}$
- $\text{sech } x = \dfrac{1}{\cosh x} = \dfrac{1}{e^x + e^{-x}}$
- $\coth x = \dfrac{\cosh x}{\sinh x} = \dfrac{e^x + e^{-x}}{e^x - e^{-x}}$
- $\text{csch } x = \dfrac{1}{\sinh x} = \dfrac{1}{e^x - e^{-x}}$

```desmos-graph
f(x) = \cosh(x)
f(x) = \sinh(x)
```

### Identities

$\cosh^2(x) - \sinh^2(x) = 1$
By dividing by $\cosh^2(x)$, we get:
$1 - \tanh^2(x) = \text{sech}^2(x)$

> The hyperbolic cosine function is also called the [**catenoid**](https://en.wikipedia.org/wiki/Catenoid#:~:text=The%20catenoid%20was%20the%20first,by%20Leonhard%20Euler%20in%201744), the shape a string takes when under the force of gravity.

### Derivatives

$\dfrac{d}{dx} \cosh(x) = \sinh(x)$
$\dfrac{d}{dx} \sinh(x) = \cosh(x)$

All other [[3.5 Derivatives of Trigonometric Functions|derivatives]] remain the same, except

$\dfrac{d}{dx} \text{sech}(x) = -\text{sech}(x) \tanh(x)$