---
tags:
  - math_171
  - limits
see also: "[[4.6 Linear Approximation and Differentials]]"
---

> A rule that's useful for finding indeterminate form limits when algebra trickery does not help.

For instance,
$$ \lim_{x \to 3} \frac{\ln{2x - 5}}{x^2 - 9} = \frac{0}{0} $$

```desmos-graph
left = 2.8; right = 3.2;
top = 0.2; bottom = -0.2;
---
f(x) = \ln(2x - 5)
f(x) = x^2 - 9
```

Using the idea of [[4.6 Linear Approximation and Differentials#Linear Approximation|linear approximation]], we can approximate $f$ and $g$ with linear functions:

$$ L(x) = f(a) + f'(a)(x - a), $$

$L_f(x) = 0 + 2(x - 3)$
$L_g(x) = 0 + 6(x - 3)$

Therefore,
$$ \lim_{x \to 3} \frac{\ln{2x - 5}}{x^2 - 3} = \lim_{x \to 3} \frac{0 + 2(x - 3)}{0 + 6(x - 3)} = \lim_{x \to 3} \frac{2}{6} = \frac{1}{3} $$

> *Theorem 4.12 L'Hôpital's Rule*
> Suppose $f$ and $g$ are differentiable on an open interval $I$ containing $a$ with $g'(x) \neq 0$ on $I$ when $x \neq a$. If $\lim_{x \to a} f(x) = \lim_{x \to a} g(x) = 0$, then
> $$ \lim_{x \to a} \frac{f(x)}{g(x)} = \lim_{x \to a} \frac{f'(x)}{g'(x)}, $$
> provided the limit on the right exists (or is $\pm \infty$). The rule also applies if $x \to a$ is replaced with $x \to \pm \infty$, $x \to a^+$, or $x \to a^-$.

- Note: l'Hôpital's Rule can be applied multiple times to arrive at a determinate form

> *Theorem 4.13 L'Hôpital's Rule $(\infty / \infty)$*
> Suppose $f$ and $g$ are differentiable on an open interval $I$ containing $a$ with $g'(x) \neq 0$ on $I$ when $x \neq a$. If $\lim_{x \to a} f(x) = \pm \infty$ and $\lim_{x \to a} g(x) = \pm \infty$, then
> $$ \lim_{x \to a} \frac{f(x)}{g(x)} = \lim_{x \to a} \frac{f'(x)}{g'(x)}, $$
> provided the limit on the right exists (or is $\pm \infty$). The rule also applies for $x \to \pm \infty$, $x \to a^+$, or $x \to a^-$.

- Note: $\frac{\infty}{\infty}$ is also indeterminate form

### Example

> Find $\lim_{x \to 0^+} (x \ln x)$.

This is another indeterminate form $(0 \cdot \infty)$.
Note that $A \cdot B = \frac{B}{\frac{1}{A}}$.
Therefore,
$\lim_{x \to 0^+} (x \ln x) = \lim_{x \to 0^+} \frac{\ln x}{\frac{1}{x}}$
$= \lim_{x \to 0^+} \frac{\frac{1}{x}}{-\frac{1}{x^2}}$
$= \lim_{x \to 0^+} -x$
$= 0$