---
tags:
  - math_171
  - derivatives
---

> *Definition: Antiderivative*
> A function $F$ is an **antiderivative** of $f$ on an interval $I$ provided $F'(x) = f(x)$, for all $x$ in $I$.

- Note: a function only has *one* derivative, but can have many antiderivatives

---

> *Theorem 4.15: The Family of Antidervatives*
> Let $F$ be any antiderivative of $f$ on an interval $I$. Then *all* the antiderivatives of $f$ on $i$ have the form $F + C$, where $C$ is an arbitrary constant.

## Notation

The **general antiderivative** of $x^3$ is
$$ x^3 + C $$
where $C$ is an arbitrary constant.

$$ \int 3x^2 \, dx = x^3 + C $$
$3x^2$ here is the **integrand**.

- Note: **general antiderivative** and **indefinite integral** are synonymous

### Example

> $$ \frac{d}{dx} (e^x) = e^x \Rightarrow \int e^x \, dx = e^x + C $$

---

> *Theorem 4.17: Constant Multiple and Sum Rules*
> **Constant Multiple Rule**: $\int cf(x) \, dx = c \int f(x) \, dx$, for real numbers $c$
> **Sum Rule**: $\int (f(x) \pm g(x)) \, dx = \int f(x) \, dx \pm \int g(x) \, dx$

### Example

> $$ \int (2e^x - sec^2(x)) \, dx $$

$= \int 2e^x \, dx - \int sec^2(x) \, dx$
$= 2e^x + C - (tan(x) + D)$
- Note: cannot use two $C$s since $C$ and $D$ are different constants

$= 2e^x - tan(x) + C - D$
$= 2e^x - tan(x) + C$
- Note: $C - D$ is the same as an arbitrary constant $C$

---

> *Theorem 4.16: Power Rule for Indefinite Integrals*
> $$ \int x^p \, dx = \frac{x^{p + 1}}{p + 1} + C, $$
> where $p \neq 1$ is a real number and $C$ is an arbitrary constant.

### Examples

> $$ f(x) = 5x^4 $$

$= \int 5x^4 \, dx$
$= 5 \int x^4 \, dx$
$= 5 \cdot (\frac{1}{5} x^5 + C)$
$= x^5 + C$


> $$ f(y) = -\frac{2}{y} $$

$= \int -2y^{-3} \, dy$
$= -2 \cdot (\frac{1}{-2} y^{-3 + 1} + C)$
$= y^{-2} + C$
$= \frac{1}{y^2} + C$

> $$ f(x) = 2 \sin(x) + 1 $$

$= \int (2 \sin(x) + 1) \, dx$
$= 2 \cdot (-\cos(x)) + x + C$
$= -2 \cos(x) + x + C$