---
tags:
  - e_e_214
created: 2024-09-11
---

## Laws

### AND

$A . 1 = A$
$A . 0 = 0$
$A . A = A$
$A . \overline A = 0$

### OR

$A + 1 = 1$
$A + 0 = A$
$A + A = A$
$A + \overline A = 1$

### Commutative

$A . B = B . A$
$A + B = B + A$

## Associative Law

$(A . B) . C = A . (B . C)$
$(A + B) + C = A + (B + C)$

### Distributive Law

$A . (B + C) = A . B + A . C$
$A + B . C = (A + B) . (A + C)$

### DeMorgan's

$\overline{A . B} = \overline A + \overline B$
$\overline{A + B} = \overline A . \overline B$

### Absorptive

$A + \overline A . B = A + B$
$A . (\overline A + B)$

Proof:
$A + \overline A . B$
$= (A + \overline A) . (A + B)$
$= 1 . (A + B)$
$= A + B$

$A . (\overline A + B)$
$= A . \overline A + A . B$
$= 0 + A . B$
$= A . B$